theories/typing/lib/list.v
@@ -1,0 +1,29 @@
+Require Import FunctionalExtensionality Equality.
+From lrust.typing Require Export type.
+From lrust.typing Require Import fixpoint mod_ty lib.option product own.
+Set Default Proof Using "Type".
+
+Section list.
+  Context `{!typeG Σ}.
+
+  Definition list_ty {A} (ty: type A) : type (list A) :=
+    fix_ty (λ ty', <{option_to_list}> (option_ty (ty * box ty')))%T.
+
+  Lemma list_subtype {A B} E L (f: A → B) ty ty' :
+    subtype E L f ty ty' → subtype E L (map f) (list_ty ty) (list_ty ty').
+  Proof.
+    move=> ?. apply fix_subtype=> *. rewrite map_via_option_map.
+    eapply subtype_trans; [apply mod_ty_out, _|]. eapply subtype_trans;
+    [|apply mod_ty_in]. by apply option_subtype, prod_subtype, box_subtype.
+  Qed.
+
+  Lemma list_eqtype {A B} E L (f: A → B) g ty ty' :
+    eqtype E L f g ty ty' → eqtype E L (map f) (map g) (list_ty ty) (list_ty ty').
+  Proof.
+    move=> ?. apply fix_eqtype=> *. rewrite map_via_option_map
+    [map g]map_via_option_map -compose_assoc. eapply eqtype_trans;
+    [|apply mod_ty_inout, _]. eapply eqtype_trans; [apply mod_ty_outin, _|].
+    by apply option_eqtype, prod_eqtype, box_eqtype.
+  Qed.
+
+End list.
